LeanCopilot/Models/Defs.lean
@@ -1,7 +1,9 @@
-import ModelCheckpointManager.Url
+import ModelCheckpointManager
 import LeanCopilot.Models.Interface
 
 set_option autoImplicit false
+
+open System (FilePath)
 
 namespace LeanCopilot
 
@@ -15,6 +17,13 @@ deriving Repr
 
 instance : Inhabited Device where
   default := .auto
+
+
+instance : ToString Device where
+  toString
+    | Device.cpu => "cpu"
+    | Device.cuda => "cuda"
+    | Device.auto => "auto"
 
 
 inductive ComputeType where
@@ -35,31 +44,57 @@ instance : Inhabited ComputeType where
   default := .auto
 
 
+instance : ToString ComputeType where
+  toString
+    | ComputeType.default => "default"
+    | ComputeType.auto => "auto"
+    | ComputeType.int8 => "int8"
+    | ComputeType.int8_float32 => "int8_float32"
+    | ComputeType.int8_float16 => "int8_float16"
+    | ComputeType.int8_bfloat16 => "int8_bfloat16"
+    | ComputeType.int16 => "int16"
+    | ComputeType.float16 => "float16"
+    | ComputeType.bfloat16 => "bfloat16"
+    | ComputeType.float32 => "float32"
+
+
+structure Tokenizer where
+  tokenize : String → Array String
+  detokenize : Array String → String
+  eosToken : String
+
+
 structure NativeModel where
   url : Url
   device : Device := default
   deviceIndex : Array UInt64 := #[0]
   computeType : ComputeType := default
+  tokenizer : Tokenizer
+
+
+def NativeModel.name (model : NativeModel) : String := model.url.name!
+
+
+def NativeModel.path (model : NativeModel) : IO FilePath :=
+  getModelDir model.url
+
+
+structure BeamSearchParams where
+  numReturnSequences : UInt64
+  beamSize : UInt64 := numReturnSequences
+  minLength : UInt64 := 1
+  maxLength : UInt64 := 1024
+  lengthPenalty : Float := 0.0
+  patience : Float := 2.0
+  temperature : Float := 1.0
 deriving Repr
 
 
-instance : Inhabited NativeModel where
-  default := {url := default}
-
-
-def NativeModel.name (model : NativeModel) : String := model.url.name
-
-
-structure NativeGenerator extends NativeModel
-deriving Repr
+structure NativeGenerator extends NativeModel where
+  params : BeamSearchParams
 
 
 structure NativeEncoder extends NativeModel
-deriving Repr
-
-
-def NativeEncoder.encode (enc : NativeEncoder) (input : String) : FloatArray :=
-  FloatArray.empty
 
 
 structure ExternalModel where
