LeanCopilot/Models/FFI.lean
@@ -1,15 +1,22 @@
+import LeanCopilot.Models.Defs
+
 namespace LeanCopilot
+
+set_option autoImplicit false
 
 namespace FFI
 
-@[extern "is_initialized"]
-opaque isInitialized : (name : @& String) → Bool
+@[extern "is_generator_initialized"]
+opaque isGeneratorInitialized : (name : @& String) → Bool
+
+@[extern "is_encoder_initialized"]
+opaque isEncoderInitialized : (name : @& String) → Bool
 
 @[extern "init_generator"]
-opaque initGenerator (name : @& String) (modelPath : @& String) (device : @& String) (computeType : @& String) (deviceIndex : @& Array UInt64) : Bool
+opaque initGenerator (name : @& String) (modelPath : @& String) (computeType : @& String) (device : @& String) (deviceIndex : @& Array UInt64) : Bool
 
 @[extern "init_encoder"]
-opaque initEncoder (name : @& String) (modelPath : @& String) (device : @& String) (computeType : @& String) (deviceIndex : @& Array UInt64) : Bool
+opaque initEncoder (name : @& String) (modelPath : @& String) (computeType : @& String) (device : @& String) (deviceIndex : @& Array UInt64) : Bool
 
 @[extern "generate"]
 opaque generate (name : @& String) (inputTokens : @& Array String) (targetPrefixTokens : @& Array String) (numReturnSequences : UInt64) (beamSize : UInt64)
@@ -39,31 +46,72 @@ end FFI
 
 namespace NativeGenerator
 
-def init (model : NativeGenerator) : Bool := sorry
+
+def init (model : NativeGenerator) : IO Bool := do
+  if FFI.isGeneratorInitialized model.name then
+    return true
+  let path := (← model.path).toString
+  let device := toString model.device
+  let computeType := toString model.computeType
+  return FFI.initGenerator model.name path computeType device model.deviceIndex
 
 
-def generate (model : NativeGenerator) (input : String) : String := "hello"
-/-
-  let inputTokens := tokenizeByt5 input true |>.toArray
-  let targetPrefixTokens := tokenizeByt5 targetPrefix false |>.toArray
-  let numReturnSequences := config.decoding.numReturnSequences
-  let beamSize := config.decoding.beamSize
-  let minLength := config.decoding.minLength
-  let maxLength := config.decoding.maxLength
-  let lengthPenalty := config.decoding.lengthPenalty
-  let patience := config.decoding.patience
-  let temperature := config.decoding.temperature
-  let tokensWithScores := FFI.ct2Generate inputTokens targetPrefixTokens numReturnSequences beamSize minLength maxLength lengthPenalty patience temperature
-  tokensWithScores.filterMap fun ((ts, s) : Array String × Float) =>
-    match detokenizeByt5 ts with
+def generate (model : NativeGenerator) (input : String) (targetPrefix : String) : IO $ Array (String × Float) := do
+  if ¬ (← init model) then
+    -- TODO: Return empty and show an error.
+    throw $ IO.userError "Failed to initialize generator"
+
+  let tokenizer := model.tokenizer
+  let inputTokens := tokenizer.tokenize input |>.push tokenizer.eosToken
+  let targetPrefixTokens := tokenizer.tokenize targetPrefix
+  let numReturnSequences := model.params.numReturnSequences
+  let beamSize := model.params.beamSize
+  let minLength := model.params.minLength
+  let maxLength := model.params.maxLength
+  let lengthPenalty := model.params.lengthPenalty
+  let patience := model.params.patience
+  let temperature := model.params.temperature
+  let tokensWithScores := FFI.generate model.name inputTokens targetPrefixTokens numReturnSequences beamSize minLength maxLength lengthPenalty patience temperature
+
+  return tokensWithScores.filterMap fun ((ts, s) : Array String × Float) =>
+    match tokenizer.detokenize ts with
     | "aesop" => none
     | t => some (t, s)
--/
+
 
 
 instance : TextToText NativeGenerator where
   generate := NativeGenerator.generate
 
+
 end NativeGenerator
+
+
+namespace NativeEncoder
+
+
+def init (model : NativeEncoder) : IO Bool := do
+  if FFI.isEncoderInitialized model.name then
+    return true
+  let path := (← model.path).toString
+  let device := toString model.device
+  let computeType := toString model.computeType
+  return FFI.initEncoder model.name path computeType device model.deviceIndex
+
+
+def encode (model : NativeEncoder) (input : String) : IO FloatArray := do
+  if ¬ (← init model) then
+    return FloatArray.mk #[]
+  let tokenizer := model.tokenizer
+  let inputTokens := tokenizer.tokenize input |>.push tokenizer.eosToken
+  return FFI.encode model.name inputTokens
+
+
+instance : TextToVec NativeEncoder where
+  encode := NativeEncoder.encode
+
+
+end NativeEncoder
+
 
 end LeanCopilot
