LeanCopilot/Models.lean
@@ -2,10 +2,3 @@ import LeanCopilot.Models.Interface
 import LeanCopilot.Models.Defs
 import LeanCopilot.Models.Registry
 import LeanCopilot.Models.FFI
-
-
-open LeanCopilot
-
-#eval (getModelRegistry : IO _)
-
-#eval generate defaultGenerator "Hi!"
