LeanCopilot/Models/Builtin.lean
@@ -1,0 +1,24 @@
+import ModelCheckpointManager
+import LeanCopilot.Models.ByT5
+
+set_option autoImplicit false
+
+namespace LeanCopilot.Builtin
+
+
+def generator : NativeGenerator := {
+  url := Url.parse! "https://huggingface.co/kaiyuy/ct2-leandojo-lean4-tacgen-byt5-small"
+  tokenizer := ByT5.tokenizer
+  params := {
+    numReturnSequences := 32
+  }
+}
+
+
+def encoder : NativeEncoder := {
+  url := Url.parse! "https://huggingface.co/kaiyuy/ct2-leandojo-lean4-retriever-byt5-small"
+  tokenizer := ByT5.tokenizer
+}
+
+
+end LeanCopilot.Builtin
