LeanCopilot/Models/Registry.lean
@@ -1,4 +1,5 @@
 import LeanCopilot.Models.Defs
+import LeanCopilot.Models.Builtin
 import Std.Data.HashMap
 
 set_option autoImplicit false
@@ -8,26 +9,15 @@ open Std
 namespace LeanCopilot
 
 
-def defaultGenerator : NativeGenerator := {
-  url := ⟨"kaiyuy", "ct2-leandojo-lean4-tacgen-byt5-small"⟩
-}
-
-
-def defaultEncoder : NativeEncoder := {
-  url := ⟨"kaiyuy", "ct2-leandojo-lean4-retriever-byt5-small"⟩
-}
-
-
 instance {α β : Type} [BEq α] [Hashable α] [Repr α] [Repr β] : Repr (HashMap α β) where
   reprPrec hm n := reprPrec hm.toList n
 
 
 structure NativeModelRegistry where
   generators : HashMap String NativeGenerator :=
-    HashMap.ofList [(defaultGenerator.name, defaultGenerator)]
+    HashMap.ofList [(Builtin.generator.name, Builtin.generator)]
   encoders : HashMap String NativeEncoder :=
-    HashMap.ofList [(defaultEncoder.name, defaultEncoder)]
-deriving Repr
+    HashMap.ofList [(Builtin.encoder.name, Builtin.encoder)]
 
 
 instance : Inhabited NativeModelRegistry where
@@ -49,7 +39,7 @@ instance : Inhabited ExternalModelRegistry where
 structure ModelRegistry where
   native : NativeModelRegistry
   external : ExternalModelRegistry
-deriving Inhabited, Repr
+deriving Inhabited
 
 
 initialize modelRegistryRef : IO.Ref ModelRegistry ← IO.mkRef default
