LeanCopilotTests/LowLevelAPIs.lean
@@ -2,6 +2,140 @@ import LeanCopilot
 
 open LeanCopilot
 
-def url := Url.parse! "https://huggingface.co/kaiyuy/ct2-leandojo-lean4-tacgen-byt5-small"
+/-
+```python
+from transformers import AutoTokenizer, AutoModelForSeq2SeqLM
 
-#eval generate model "a b : ℕ\n⊢ a + b = b + a"
+tokenizer = AutoTokenizer.from_pretrained("kaiyuy/leandojo-lean4-tacgen-byt5-small")
+model = AutoModelForSeq2SeqLM.from_pretrained("kaiyuy/leandojo-lean4-tacgen-byt5-small")
+
+state = "n : ℕ\n⊢ gcd n n = n"
+tokenized_state = tokenizer(state, return_tensors="pt")
+
+# Generate a single tactic.
+tactic_ids = model.generate(tokenized_state.input_ids, max_length=1024)
+tactic = tokenizer.decode(tactic_ids[0], skip_special_tokens=True)
+print(tactic, end="\n\n")
+
+# Generate multiple tactics via beam search.
+tactic_candidates_ids = model.generate(
+    tokenized_state.input_ids,
+    max_length=1024,
+    num_beams=4,
+    length_penalty=0.0,
+    do_sample=False,
+    num_return_sequences=4,
+    early_stopping=False,
+)
+tactic_candidates = tokenizer.batch_decode(
+    tactic_candidates_ids, skip_special_tokens=True
+)
+for tac in tactic_candidates:
+    print(tac)
+```
+-/
+
+
+def model₁ : NativeGenerator := {
+  url := Url.parse! "https://huggingface.co/kaiyuy/ct2-leandojo-lean4-tacgen-byt5-small"
+  tokenizer := ByT5.tokenizer
+  params := {
+    numReturnSequences := 1
+  }
+}
+
+#eval generate model₁ "n : ℕ\n⊢ gcd n n = n"
+
+
+def model₁' : NativeGenerator := {model₁ with params := {numReturnSequences := 4}}
+
+#eval generate model₁' "n : ℕ\n⊢ gcd n n = n"
+
+
+def model₁'' : NativeGenerator := {
+  url := Url.parse! "https://huggingface.co/kaiyuy/ct2-byt5-small"
+  tokenizer := ByT5.tokenizer
+  params := {
+    numReturnSequences := 1
+  }
+}
+
+#eval generate model₁'' "n : ℕ\n⊢ gcd n n = n"
+
+
+/-
+```python
+from transformers import AutoTokenizer, T5EncoderModel
+
+tokenizer = AutoTokenizer.from_pretrained("kaiyuy/leandojo-lean4-retriever-byt5-small")
+model = T5EncoderModel.from_pretrained("kaiyuy/leandojo-lean4-retriever-byt5-small")
+
+state = "n : ℕ\n⊢ gcd n n = n"
+tokenized_state = tokenizer(state, return_tensors="pt")
+hidden_state = model(tokenized_state.input_ids).last_hidden_state
+feature = hidden_state.mean(dim=1).squeeze()
+print(feature)
+```
+-/
+
+
+def model₂ : NativeEncoder := {
+  url := Url.parse! "https://huggingface.co/kaiyuy/ct2-leandojo-lean4-retriever-byt5-small"
+  tokenizer := ByT5.tokenizer
+}
+
+#eval encode model₂ "n : ℕ\n⊢ gcd n n = n"
+
+
+/-
+```python
+from transformers import AutoTokenizer, AutoModelForCausalLM
+
+tokenizer = AutoTokenizer.from_pretrained("EleutherAI/llemma_7b")
+model = AutoModelForCausalLM.from_pretrained("EleutherAI/llemma_7b")
+
+state = "n : ℕ\n⊢ gcd n n = n"
+tokenized_state = tokenizer(state, return_tensors="pt")
+
+# Generate a single tactic.
+tactic_ids = model.generate(tokenized_state.input_ids, max_length=32)
+tactic = tokenizer.decode(tactic_ids[0], skip_special_tokens=True)
+print(tactic, end="\n\n")
+
+# Generate multiple tactics via beam search.
+tactic_candidates_ids = model.generate(
+    tokenized_state.input_ids,
+    max_length=32,
+    num_beams=2,
+    length_penalty=0.0,
+    do_sample=False,
+    num_return_sequences=2,
+    early_stopping=False,
+)
+tactic_candidates = tokenizer.batch_decode(
+    tactic_candidates_ids, skip_special_tokens=True
+)
+for tac in tactic_candidates:
+    print(tac)
+```
+-/
+
+def model₃ : NativeGenerator := {
+  url := Url.parse! "https://huggingface.co/EleutherAI/llemma_7b"
+  tokenizer := sorry
+  params := {
+    numReturnSequences := 1
+  }
+}
+
+#eval generate model₃ "n : ℕ\n⊢ gcd n n = n"
+
+
+def model₃' : NativeGenerator := {model₃ with params := {numReturnSequences := 2}}
+
+#eval generate model₃' "n : ℕ\n⊢ gcd n n = n"
+
+
+/-
+TODO: A dummy model in lean.
+-/
